\subsection*{Question 1}

\textbf{a)} Examine $\mu(t)$ and its relative change over time $\frac{1}{\mu(t)} \odv{\mu(t)}{t}$ in order to provide an interpretation for each parameter of (\autoref{eq:mu_beta}).

\begin{center}\rule{6cm}{0.4pt}\end{center}

Let's compute the derivative first,
\begin{align*}
	\odv{\mu(t)}{t} 
		&= \mu(t) \odv{}{t} \left( \frac{\beta_1}{\beta_2} (1 - e^{-\beta_2 t}) \right) \\
		&=  \frac{\beta_1}{\beta_2} \mu(t) e^{-\beta_2 t} \beta_2 \\
		&= \beta_1 \mu(t) e^{-\beta_2 t}
\end{align*}

We then have,
\begin{equation*}
	\frac{1}{\mu(t)} \odv{\mu(t)}{t} = \beta_1 e^{-\beta_2 t}
\end{equation*}

\textbf{b)} Provide the formulas connecting the $\beta_k$ and $\alpha_k$ parameters.

\begin{center}\rule{6cm}{0.4pt}\end{center}

Let's compute the relative change over time of \autoref{eq:mu_alpha},
\begin{align*}
	\odv{\mu(t)}{t} = \mu(t) \alpha_1 \alpha_2 e^{-\alpha_2 t}
\end{align*}

we then have,
\begin{align*}
	\frac{1}{\mu(t)} \odv{\mu(t)}{t} = \alpha_1 \alpha_2 e^{-\alpha_2 t}
\end{align*}

Computing the limits toward zero for the two relative changes, we get,
\begin{equation} \label{eq:rel-changes-lim-zero}
	\beta_1 = \alpha_1 \alpha_2
\end{equation}

Computing the limits toward zero for the two $\mu(t)$ formulas we get,
\begin{equation}
	\ln\left( \frac{\beta_0}{\alpha_0} \right) = -\alpha_1
\end{equation}

We can then compute the limits toward infinity for the two $\mu(t)$ formulas,
\begin{equation}
	\ln\left(  \frac{\beta_0}{\alpha_0} \right) = - \frac{\beta_1}{\beta_2}
\end{equation}

We then get, 
\begin{equation}
	\alpha_1 = \frac{\beta_1}{\beta_2}
\end{equation}
Inserting into \autoref{eq:rel-changes-lim-zero}, it gives us,
\begin{equation}
	\beta_2 = \alpha_2
\end{equation}

We can then compare the two formulas for $\mu(t)$,
\begin{align*}
	\beta_1 e^{-\beta_2 t} 
		&= \alpha_1 \beta_2 e^{-\beta_2 t} \\
	\iff \beta_1 
		&= \alpha_1 \beta_2 = \alpha_1 \alpha_2
\end{align*}

And compare the twos relative changes,
\begin{align*}
	\beta_0 \exp\left( \alpha_1 (1 - e^{-\alpha_2 t}) \right)
		&= \alpha_0 \exp(-\alpha_1 e^{-\alpha_2 t}) \\
	\iff \beta_0 e^{\alpha_1} 
		&= \alpha_0 \\
	\iff \beta_0
		&= \frac{\alpha_0}{e^{\alpha_1}}
\end{align*}

To summarize, we found the following relations linking the $\alpha_k$ and $\beta_k$,
\begin{equation}
	\begin{cases}
		\beta_0 &= \frac{\alpha_0}{e^{\alpha_1}} \\
		\beta_1 &= \alpha_1 \alpha_2 \\
		\beta_2 &= \alpha_2
	\end{cases}
\end{equation}